code/experimental/pkcs/Spec/Hacl.PKCS11.Lemmas.LowLevel.fst
@@ -1,0 +1,12 @@
+module Hacl.PKCS11.Lemmas.LowLevel
+
+open FStar.Seq
+
+
+assume val lemmaFromListToSequence: #a: Type0 
+  -> l: list a 
+  -> Lemma
+  (ensures (
+    forall (i: nat). i < List.Tot.length l ==>
+    index (seq_of_list l) i == List.Tot.index l i)
+  )
